theories/ftlr/Subseg.v
@@ -51,8 +51,7 @@ Section fundamental.
           -∗ (∀ r1 : RegName, ⌜r1 ≠ PC⌝ → (fixpoint interp1) (a0 !r! r1))
           -∗ registers_mapsto (<[PC:=inr (a1, a2, a3, a4)]> a0)
           -∗ na_own logrel_nais ⊤
-          -∗ ⌜a1 = RX ∨ a1 = RWX⌝
-             → □ (fixpoint interp1) (inr (a1, a2, a3, a4)) -∗ interp_conf)) -∗
+          -∗ □ (fixpoint interp1) (inr (a1, a2, a3, a4)) -∗ interp_conf)) -∗
       (fixpoint interp1) (inr (p, b, e, a)) -∗
       (fixpoint interp1) (inr (p, b', e', a)).
   Proof.
